Add more inversions

language_formalisation/type_system/subtyping_lemmas.v
@@ -10,29 +10,31 @@ Require Import syntax declarational wellfounded_lemmas.
 
 Ltac inv H := inversion H; clear H; subst.
 
+
 (* ========================== Auxiliary Lemmas ========================== *)
+
 
 Lemma sig_subtype_gets_Some Σ Σ' op A B :
   sig_subtype Σ Σ' -> get_op_type Σ op = Some (A, B) -> exists A' B', 
   get_op_type Σ' op = Some (A', B') /\ vsubtype A' A /\ vsubtype B B'.
 Proof.
-intros sty gets. induction sty.
-+ simpl in gets. discriminate.
-+ simpl in gets. destruct (op == op0).
-  - injection gets. intros. subst. exists A'. exists B'.
-    constructor. assumption. constructor; assumption.
-  - apply IHsty in gets. assumption.
+intros sty gets. induction sty; simpl in gets. discriminate.
+destruct (op == op0).
+- injection gets. intros. subst. exists A'. exists B'.
+  constructor. assumption. constructor; assumption.
+- apply IHsty in gets. assumption.
 Qed.
+
 
 Lemma sig_subtype_gets_None Σ Σ' op :
   sig_subtype Σ Σ' -> get_op_type Σ' op = None -> get_op_type Σ op = None.
 Proof.
-intros sty gets. induction sty.
-+ simpl. reflexivity.
-+ simpl. destruct (op == op0).
-  - rewrite e in *. rewrite gets in H0. discriminate.
-  - apply IHsty. assumption.
+intros sty gets. induction sty; simpl. reflexivity.
+destruct (op == op0).
+- rewrite e in *. rewrite gets in H. discriminate.
+- apply IHsty. assumption.
 Qed.
+
 
 Lemma sig_subtype_extend Σ Σ' op A B :
   sig_subtype Σ Σ' -> wf_sig (SigU Σ' op A B) -> sig_subtype Σ (SigU Σ' op A B).
@@ -42,43 +44,39 @@ induction H.
 + apply SigØsubty.
 + eapply SigUsubty.
   - apply IHsig_subtype. assumption.
-  - assumption.
   - inv H0. simpl. destruct (op0 == op). 
-    * rewrite e in *. rewrite H2 in H10. discriminate.
-    * exact H2.
+    * rewrite e in *. rewrite H1 in H9. discriminate.
+    * exact H1.
   - assumption.
   - assumption.
 Qed.
 
+
 Lemma sig_subtype_sigempty Σ : sig_subtype Σ SigØ -> Σ = SigØ.
 Proof.
-intro subty.
-inv subty. reflexivity.
-simpl in H1. discriminate.
+intro subty. inv subty. reflexivity. simpl in H1. discriminate.
 Qed.
+
 
 Lemma eqs_subtype_extend E E' Σ Γ Z T1 T2 :
   eqs_subtype E E' -> wf_eqs (EqsU E' Γ Z T1 T2) Σ ->
   eqs_subtype E (EqsU E' Γ Z T1 T2).
 Proof.
-intros.
-induction H.
-+ apply EqsØsubty.
-+ eapply EqsUsubty.
-  - apply IHeqs_subtype. assumption.
-  - simpl. right. assumption.
+intros. induction H.
+apply EqsØsubty.
+eapply EqsUsubty.
+- apply IHeqs_subtype. assumption.
+- simpl. right. assumption.
 Qed.
+
 
 Lemma eqs_subtype_contains E E' Γ Z T1 T2 :
   eqs_subtype E E' -> eqs_contain_eq E Γ Z T1 T2 -> eqs_contain_eq E' Γ Z T1 T2.
 Proof.
-intros sty gets. induction sty.
-+ simpl in gets. destruct gets.
-+ simpl in gets. destruct gets.
-  - destruct H0 as [a [b [c ]]]. subst. assumption.
-  - apply IHsty. assumption.
+intros sty gets. induction sty; simpl in gets; destruct gets.
+- destruct H0 as [a [b [c ]]]. subst. assumption.
+- apply IHsty. assumption.
 Qed.
-
 
 
 (* ========================== Basic Properties ========================== *)
@@ -106,7 +104,6 @@ intros; induction Σ.
 + apply SigØsubty.
 + eapply SigUsubty.
   - apply sig_subtype_extend. apply IHΣ. inv H. assumption. assumption.
-  - inv H. assumption.
   - simpl. destruct (o==o). reflexivity. destruct n. reflexivity.
   - apply vsubtype_refl. inv H. assumption.
   - apply vsubtype_refl. inv H. assumption.
@@ -116,9 +113,12 @@ intros; induction Σ.
   - apply IHE. assumption.
   - apply WfEqsU. exact H6. assumption. assumption.
   - simpl. left. auto.
-}{induction Γ; intros.
-+ apply CtxØsubty.
-+ apply CtxUsubty; inv H. apply IHΓ. assumption. apply vsubtype_refl. assumption.
+}
+{clear csubtype_refl sig_subty_refl eqs_subty_refl ctx_subty_refl.
+induction Γ; intros.
+apply CtxØsubty.
+apply CtxUsubty; inv H. apply IHΓ. assumption. 
+apply vsubtype_refl. assumption.
 }
 Qed.
 
@@ -138,174 +138,150 @@ Qed.
 
 (* Weird notation for SPEED! *)
 Fixpoint vsubtype_trans A1 A2 A3 
-  (A12 : vsubtype A1 A2) {struct A12} : 
-  vsubtype A2 A3 -> 
-  vsubtype A1 A3
+  (A12 : vsubtype A1 A2) {struct A12} : vsubtype A2 A3 -> vsubtype A1 A3
+
 with vsubtype_trans_rev A1 A2 A3
-  (A21 : vsubtype A2 A1) {struct A21} : 
-  vsubtype A3 A2 ->
-  vsubtype A3 A1
+  (A21 : vsubtype A2 A1) {struct A21} : vsubtype A3 A2 -> vsubtype A3 A1
+
 with csubtype_trans C1 C2 C3
-  (C12 : csubtype C1 C2) {struct C12} : 
-  csubtype C2 C3 -> 
-  csubtype C1 C3
+  (C12 : csubtype C1 C2) {struct C12} : csubtype C2 C3 -> csubtype C1 C3
+
 with csubtype_trans_rev C1 C2 C3 
-  (C21 : csubtype C2 C1) {struct C21} : 
-  csubtype C3 C2 -> 
-  csubtype C3 C1
+  (C21 : csubtype C2 C1) {struct C21} : csubtype C3 C2 -> csubtype C3 C1
+
 with sig_subtype_trans Σ1 Σ2 Σ3 
-  (S12 : sig_subtype Σ1 Σ2) {struct S12} : 
-  sig_subtype Σ2 Σ3 -> 
+  (S12 : sig_subtype Σ1 Σ2) {struct S12} : sig_subtype Σ2 Σ3 -> 
   sig_subtype Σ1 Σ3
+
 with sig_subtype_trans_rev Σ1 Σ2 Σ3
-  (S21 : sig_subtype Σ2 Σ1) {struct S21} :
-  sig_subtype Σ3 Σ2 -> 
+  (S21 : sig_subtype Σ2 Σ1) {struct S21} : sig_subtype Σ3 Σ2 -> 
   sig_subtype Σ3 Σ1
-with nema_problema_lemma op A' A B B' Σ1 Σ2
-  (S12 : sig_subtype Σ1 Σ2) {struct S12} :
-  get_op_type Σ1 op = Some (A', B') ->
-  vsubtype A' A -> vsubtype B B' ->
-  exists A'' B'', get_op_type Σ2 op = Some (A'', B'') /\
-  vsubtype A'' A /\ vsubtype B B''.
+
+with get_op_trans op A' A B B' Σ1 Σ2 (S12 : sig_subtype Σ1 Σ2) {struct S12} :
+  get_op_type Σ1 op = Some (A', B') -> vsubtype A' A -> vsubtype B B' ->
+  exists A'' B'', 
+  get_op_type Σ2 op = Some (A'', B'') /\ vsubtype A'' A /\ vsubtype B B''.
 Proof.
 {
-clear sig_subtype_trans sig_subtype_trans_rev.
-intros A23; destruct A12; try assumption; 
-inv A23. 
+clear sig_subtype_trans sig_subtype_trans_rev get_op_trans.
+intros A23; destruct A12; try assumption; inv A23. 
 + apply VsubtyTyΣ.
-  - eapply vsubtype_trans. exact A12_1. all: assumption.
-  - eapply vsubtype_trans. exact A12_2. all: assumption.
+  - eapply vsubtype_trans. exact A12_1. assumption.
+  - eapply vsubtype_trans. exact A12_2. assumption.
 + apply VsubtyTyΠ.
-  - eapply vsubtype_trans. exact A12_1. all: assumption.
-  - eapply vsubtype_trans. exact A12_2. all: assumption.
+  - eapply vsubtype_trans. exact A12_1. assumption.
+  - eapply vsubtype_trans. exact A12_2. assumption.
 + apply VsubtyFun.
-  - eapply vsubtype_trans_rev. exact A12. all: assumption. 
-  - eapply csubtype_trans. exact H. all: assumption.
+  - eapply vsubtype_trans_rev. exact A12. assumption. 
+  - eapply csubtype_trans. exact H. assumption.
 + apply VsubtyHandler.
-  - eapply csubtype_trans_rev. exact H. all: assumption. 
-  - eapply csubtype_trans. exact H0. all: assumption.
+  - eapply csubtype_trans_rev. exact H. assumption. 
+  - eapply csubtype_trans. exact H0. assumption.
 }{
-clear sig_subtype_trans sig_subtype_trans_rev.
-intros A32; destruct A21; try assumption;
-inv A32. 
+clear sig_subtype_trans sig_subtype_trans_rev get_op_trans.
+intros A32; destruct A21; try assumption; inv A32. 
 + apply VsubtyTyΣ.
-  - eapply vsubtype_trans_rev. exact A21_1. all: assumption.
-  - eapply vsubtype_trans_rev. exact A21_2. all: assumption.
+  - eapply vsubtype_trans_rev. exact A21_1. assumption.
+  - eapply vsubtype_trans_rev. exact A21_2. assumption.
 + apply VsubtyTyΠ.
-  - eapply vsubtype_trans_rev. exact A21_1. all: assumption.
-  - eapply vsubtype_trans_rev. exact A21_2. all: assumption.
+  - eapply vsubtype_trans_rev. exact A21_1. assumption.
+  - eapply vsubtype_trans_rev. exact A21_2. assumption.
 + apply VsubtyFun.
-  - eapply vsubtype_trans. exact A21. all: assumption. 
-  - eapply csubtype_trans_rev. exact H. all: assumption.
+  - eapply vsubtype_trans. exact A21. assumption. 
+  - eapply csubtype_trans_rev. exact H. assumption.
 + apply VsubtyHandler.
-  - eapply csubtype_trans. exact H. all: assumption. 
-  - eapply csubtype_trans_rev. exact H0. all: assumption.
+  - eapply csubtype_trans. exact H. assumption. 
+  - eapply csubtype_trans_rev. exact H0. assumption.
 }{
 clear vsubtype_trans_rev csubtype_trans csubtype_trans_rev.
-clear sig_subtype_trans_rev.
-intros C23; destruct C12. 
-inv C23. 
-apply Csubty.
-- eapply vsubtype_trans. exact H. all: assumption.
-- eapply sig_subtype_trans. exact H0. all: assumption.
-- eapply eqs_subtype_trans. all: eauto.
+clear sig_subtype_trans_rev get_op_trans.
+intros C23; destruct C12. inv C23. apply Csubty.
+- eapply vsubtype_trans. exact H. assumption.
+- eapply sig_subtype_trans. exact H0. assumption.
+- eapply eqs_subtype_trans. exact H1. assumption.
 }{
 clear vsubtype_trans csubtype_trans csubtype_trans.
-clear sig_subtype_trans.
-intros C32; destruct C21. 
-inv C32. 
-apply Csubty.
-- eapply vsubtype_trans_rev. exact H. all: assumption.
-- eapply sig_subtype_trans_rev. exact H0. all: assumption.
-- eapply eqs_subtype_trans. all: eauto.
+clear sig_subtype_trans get_op_trans.
+intros C32; destruct C21. inv C32. apply Csubty.
+- eapply vsubtype_trans_rev. exact H. assumption.
+- eapply sig_subtype_trans_rev. exact H0. assumption.
+- eapply eqs_subtype_trans. exact H8. assumption.
 }{
-clear csubtype_trans csubtype_trans_rev.
+clear csubtype_trans csubtype_trans_rev sig_subtype_trans_rev.
 intros S23. destruct S12.
 apply SigØsubty.
-apply (sig_subtype_gets_Some Σ' Σ3) in H0 as H0'. destruct H0' as [A'' [B'' [g]]].
-eapply SigUsubty.
-+ eapply sig_subtype_trans. exact S12. all : assumption.
-+ assumption.
-+ exact g.
+apply (sig_subtype_gets_Some Σ' Σ3) in H as H'.
+destruct H' as [A'' [B'' [g]]]. eapply SigUsubty.
+2 : exact g. all: try assumption.
++ eapply sig_subtype_trans. exact S12. assumption.
 + clear sig_subtype_trans vsubtype_trans.
-  destruct H3. eapply vsubtype_trans_rev. exact H1.
-  - assumption.
+  destruct H2. eapply vsubtype_trans_rev. exact H0. assumption.
 + clear sig_subtype_trans vsubtype_trans_rev.
-  destruct H3. eapply vsubtype_trans. exact H2.
-  - assumption.
-+ assumption.
+  destruct H2. eapply vsubtype_trans. exact H1. assumption.
 }{
-clear csubtype_trans csubtype_trans_rev.
-clear sig_subtype_trans.
+clear csubtype_trans csubtype_trans_rev sig_subtype_trans.
 intros S32. destruct S21.
 apply sig_subtype_sigempty in S32. subst. apply SigØsubty.
 induction Σ3.
 apply SigØsubty.
-
-inv S32. simpl in H10. destruct (o==op).
-+ injection H10. intros. subst. eapply SigUsubty.
+inv S32. simpl in H8. destruct (o==op).
++ injection H8. intros. subst. eapply SigUsubty.
   - apply IHΣ3. assumption.
-  - assumption.
-  - exact H0.
-  - eapply vsubtype_trans. exact H1. assumption.
-  - eapply vsubtype_trans_rev. exact H2. assumption.
-+ eapply nema_problema_lemma in H10 as gets'. 
-  2:exact S21. 2:exact H11. 2:exact H12.
-  destruct gets' as [A'' [B'' [gets']]]. eapply SigUsubty.
-  - apply IHΣ3. assumption.
-  - assumption.
-  - exact gets'.
-  - destruct H3. assumption.
-  - destruct H3. assumption.
+  - exact H.
+  - eapply vsubtype_trans. exact H0. assumption.
+  - eapply vsubtype_trans_rev. exact H1. assumption.
++ eapply get_op_trans in H8 as gets'.
+  2:exact S21. 2:exact H9. 2:exact H10.
+  destruct gets' as [A'' [B'' [gets' [styA'']]]]. eapply SigUsubty.
+  2: exact gets'. all: try assumption.
+  apply IHΣ3. assumption.
 }{
 clear csubtype_trans csubtype_trans_rev.
-clear sig_subtype_trans sig_subtype_trans_rev.
-clear nema_problema_lemma.
+clear sig_subtype_trans sig_subtype_trans_rev get_op_trans.
 intros. revert H. induction S12; intros gets.
 simpl in gets. discriminate.
 simpl in *. destruct (op==op0).
 + injection gets. intros. subst.
   exists A'0. exists B'0. constructor. assumption. constructor.
-  eapply vsubtype_trans. exact H3. assumption.
-  eapply vsubtype_trans_rev. exact H4. assumption.
+  eapply vsubtype_trans. exact H2. assumption.
+  eapply vsubtype_trans_rev. exact H3. assumption.
 + apply IHS12. assumption.
 }
 Qed.
 
 
-Fixpoint ctx_subtype_get Γ Γ' A num
-  (ctx_sty : ctx_subtype Γ Γ') {struct ctx_sty}:
+Fixpoint ctx_subtype_get Γ Γ' A num (csty : ctx_subtype Γ Γ') {struct csty}:
   get_vtype Γ num = Some A -> 
   exists A', get_vtype Γ' num = Some A' /\ vsubtype A A'.
 Proof.
-revert num. induction ctx_sty.
+revert num. induction csty. clear ctx_subtype_get.
 + intros num H. simpl in H. discriminate.
-+ intros num get.
-  destruct num.
-  - clear IHctx_sty. simpl in *. injection get. intros. subst. exists A'.
++ intros num get. destruct num.
+  - clear IHcsty. simpl in *. injection get. intros. subst. exists A'.
     constructor. reflexivity. assumption.
-  - simpl in *. eapply IHctx_sty.  clear IHctx_sty. exact get.
+  - simpl in *. eapply IHcsty. exact get.
 Qed.
 
-Fixpoint ctx_subtype_get_reverse Γ Γ' A num
-  (ctx_sty : ctx_subtype Γ' Γ) {struct ctx_sty}:
+
+Fixpoint ctx_subtype_get_rev Γ Γ' A num (csty : ctx_subtype Γ' Γ) {struct csty}:
   get_vtype Γ num = Some A -> 
   exists A', get_vtype Γ' num = Some A' /\ vsubtype A' A.
 Proof.
-revert num. induction ctx_sty.
+revert num. induction csty. clear ctx_subtype_get_rev.
 + intros num H. simpl in H. discriminate.
-+ intros num get.
-  destruct num.
-  - clear IHctx_sty. simpl in *. injection get. intros. subst. exists A0.
++ intros num get. destruct num.
+  - clear IHcsty. simpl in *. injection get. intros. subst. exists A0.
     constructor. reflexivity. assumption.
-  - simpl in *. eapply IHctx_sty.  clear IHctx_sty. exact get.
+  - simpl in *. eapply IHcsty. exact get.
 Qed.
 
 
 Fixpoint ctx_subtype_vtype Γ Γ' v A (types : has_vtype Γ v A) {struct types}:
   wf_ctx Γ' -> ctx_subtype Γ' Γ  -> has_vtype Γ' v A
+
 with ctx_subtype_ctype Γ Γ' c C (types : has_ctype Γ c C ) {struct types}:
   wf_ctx Γ' -> ctx_subtype Γ' Γ -> has_ctype Γ' c C
+
 with ctx_subtype_htype Γ Γ' h Σ D (types : has_htype Γ h Σ D) {struct types}:
   wf_ctx Γ' -> ctx_subtype Γ' Γ -> has_htype Γ' h Σ D.
 Proof.
@@ -314,17 +290,16 @@ intros wf ctxsty.
 destruct types. induction H1; apply TypeV; try assumption.
 + apply TypeUnit.
 + apply TypeInt.
-+ apply (ctx_subtype_get_reverse _ _ A num) in ctxsty. destruct ctxsty as [A' [gets]]. 
++ apply (ctx_subtype_get_rev _ _ A num) in ctxsty.
+  destruct ctxsty as [A' [gets]]. 
   eapply TypeVSubtype.
   - apply TypeV. assumption. apply ctx_gets_wf in gets as wfA'.
     exact wfA'. assumption. apply TypeVar. assumption.
   - assumption.
   - assumption.
-+ apply TypePair.
-  - eapply (ctx_subtype_vtype Γ Γ'); assumption.
-  - eapply (ctx_subtype_vtype Γ Γ'); assumption.
-+ apply TypeInl. eapply (ctx_subtype_vtype Γ Γ'); assumption.
-+ apply TypeInr. eapply (ctx_subtype_vtype Γ Γ'); assumption.
++ apply TypePair; apply (ctx_subtype_vtype Γ Γ'); assumption.
++ apply TypeInl. apply (ctx_subtype_vtype Γ Γ'); assumption.
++ apply TypeInr. apply (ctx_subtype_vtype Γ Γ'); assumption.
 + apply TypeFun. eapply ctx_subtype_ctype.
   - exact H1.
   - apply WfCtxU. assumption. inv H0. assumption.
@@ -332,7 +307,8 @@ destruct types. induction H1; apply TypeV; try assumption.
 + apply TypeHandler. eapply ctx_subtype_ctype.
   - exact H1.
   - apply WfCtxU. assumption. inv H0. inv H5. assumption.
-  - apply CtxUsubty. exact ctxsty. apply vsubtype_refl. inv H0. inv H5.           assumption.
+  - apply CtxUsubty. exact ctxsty. apply vsubtype_refl.
+    inv H0. inv H5. assumption.
   - eapply (ctx_subtype_htype Γ Γ'); assumption.
 + eapply TypeVSubtype. 2 : exact H2.
   eapply (ctx_subtype_vtype Γ Γ'); assumption.
@@ -349,14 +325,12 @@ destruct types. induction H1; apply TypeC; try assumption.
       all: inv H2; inv H3; inv H7; apply vsubtype_refl; assumption.
 + eapply TypeΣMatch.
   - eapply ctx_subtype_vtype.  exact H1. all: assumption.
-  - eapply ctx_subtype_ctype.
-    * exact H2.
-    * inv H2. inv H4. apply WfCtxU; assumption.
-    * apply CtxUsubty. exact ctxsty. apply vsubtype_refl. inv H2. inv H4. auto.
-  - eapply ctx_subtype_ctype.
-    * exact H3.
-    * inv H3. inv H4. apply WfCtxU; assumption.
-    * apply CtxUsubty. exact ctxsty. apply vsubtype_refl. inv H3. inv H4. auto.
+  - eapply ctx_subtype_ctype. exact H2. all: inv H2; inv H4. 
+    * apply WfCtxU; assumption.
+    * apply CtxUsubty. exact ctxsty. apply vsubtype_refl. assumption.
+  - eapply ctx_subtype_ctype. exact H3. all: inv H3; inv H4. 
+    * apply WfCtxU; assumption.
+    * apply CtxUsubty. exact ctxsty. apply vsubtype_refl. assumption.
 + eapply TypeDoBind.
   - eapply ctx_subtype_ctype. exact H1. all: assumption.
   - inv H1. inv H4. eapply ctx_subtype_ctype.
@@ -370,17 +344,13 @@ destruct types. induction H1; apply TypeC; try assumption.
   - eapply ctx_subtype_vtype. exact H1. all: assumption.
   - eapply ctx_subtype_ctype. exact H2. all: assumption.
 + eapply TypeLetRec.
-  - eapply ctx_subtype_ctype.
-    * exact H1.
-    * inv H2. inv H3. apply WfCtxU. apply WfCtxU.
-      assumption. inv H8. exact H6. exact H8.
+  - eapply ctx_subtype_ctype. exact H1. all: inv H2; inv H3.
+    * apply WfCtxU. apply WfCtxU. assumption. inv H8. exact H6. exact H8.
     * apply CtxUsubty. apply CtxUsubty. exact ctxsty.
-      apply vsubtype_refl. inv H2. inv H3. inv H8. assumption.
-      apply vsubtype_refl. inv H2. inv H3. assumption.
-  - eapply ctx_subtype_ctype.
-    * exact H2.
-    * inv H2. inv H3. apply WfCtxU; assumption.
-    * apply CtxUsubty. exact ctxsty. apply vsubtype_refl. inv H2. inv H3. auto.
+      apply vsubtype_refl. inv H8. assumption. apply vsubtype_refl. assumption.
+  - eapply ctx_subtype_ctype. exact H2. all: inv H2; inv H3.
+    * apply WfCtxU; assumption.
+    * apply CtxUsubty. exact ctxsty. apply vsubtype_refl. assumption.
 + eapply TypeOp.
   exact H1. eapply ctx_subtype_vtype. exact H2. assumption. assumption.
   eapply ctx_subtype_ctype. exact H3. all: inv H3; inv H4.
@@ -402,46 +372,44 @@ destruct types. induction H2; apply TypeH; try assumption.
 }
 Qed.
 
+
 (* ========================== Subtype Shapes ========================== *)
 
-Fixpoint subty_shape_pair A B C :
-  vsubtype C (TyΠ A B) -> 
+
+Fixpoint subty_shape_pair A B C : vsubtype C (TyΠ A B) -> 
   exists A' B', C = (TyΠ A' B') /\ vsubtype A' A /\ vsubtype B' B.
 Proof.
-intro orig.
-inv orig. exists A0. exists B0.
+intro orig. inv orig. exists A0. exists B0.
 constructor. reflexivity. constructor; assumption.
 Qed.
 
-Fixpoint subty_shape_sum A B C :
-  vsubtype C (TyΣ A B) -> 
+
+Fixpoint subty_shape_sum A B C : vsubtype C (TyΣ A B) -> 
   exists A' B', C = (TyΣ A' B') /\ vsubtype A' A /\ vsubtype B' B.
 Proof.
-intro orig.
-inv orig. exists A0. exists B0.
+intro orig. inv orig. exists A0. exists B0.
 constructor. reflexivity. constructor; assumption.
 Qed.
 
-Fixpoint subty_shape_fun A B C :
-  vsubtype C (TyFun A B) -> 
+
+Fixpoint subty_shape_fun A B C : vsubtype C (TyFun A B) -> 
   exists A' B', C = (TyFun A' B') /\ vsubtype A A' /\ csubtype B' B.
 Proof.
-intro orig.
-inv orig. exists A0. exists C0.
+intro orig. inv orig. exists A0. exists C0.
 constructor. reflexivity. constructor; assumption.
 Qed.
 
-Fixpoint subty_shape_handler A B C :
-  vsubtype C (TyHandler A B) -> 
+
+Fixpoint subty_shape_handler A B C : vsubtype C (TyHandler A B) -> 
   exists A' B', C = (TyHandler A' B') /\ csubtype A A' /\ csubtype B' B.
 Proof.
-intro orig.
-inv orig. exists C0. exists D.
+intro orig. inv orig. exists C0. exists D.
 constructor. reflexivity. constructor; assumption.
 Qed.
 
 
 (* ========================== Value Shapes ========================== *)
+
 
 (* Pair *)
 Fixpoint shape_pair_full Γ v A B ty (orig : has_vtype Γ v ty) {struct orig} :
@@ -467,6 +435,7 @@ destruct orig. destruct H1; try discriminate.
     * eapply TypeVSubtype. exact H3. assumption.
     * eapply TypeVSubtype. exact H4. assumption.
 Qed.
+
 
 Lemma shape_pair Γ v1 v2 A B :
   has_vtype Γ (Pair v1 v2) (TyΠ A B) ->  
@@ -508,6 +477,7 @@ destruct orig. destruct H1; try discriminate.
       exact H3. destruct H2. assumption.
 Qed.
 
+
 Lemma shape_sum_inl Γ v A B :
   has_vtype Γ (Inl v) (TyΣ A B) -> has_vtype Γ v A.
 Proof.
@@ -515,10 +485,11 @@ intro orig.
 apply (shape_sum_full _ _ A B) in orig as shape. 2: reflexivity.
 destruct shape.
 + destruct H as [name [num]]. discriminate.
-+ destruct H.
-  - destruct H. destruct H. inv H. assumption.
-  - destruct H. destruct H. discriminate.
++ destruct H; destruct H; destruct H.
+  - inv H. assumption.
+  - discriminate.
 Qed.
+
 
 Lemma shape_sum_inr Γ v A B :
   has_vtype Γ (Inr v) (TyΣ A B) -> has_vtype Γ v B.
@@ -527,9 +498,9 @@ intro orig.
 apply (shape_sum_full _ _ A B) in orig as shape. 2: reflexivity.
 destruct shape.
 + destruct H as [name [num]]. discriminate.
-+ destruct H.
-  - destruct H. destruct H. discriminate.
-  - destruct H. destruct H. inv H. assumption.
++ destruct H; destruct H; destruct H.
+  - discriminate.
+  - inv H. assumption.
 Qed.
 
 
@@ -567,17 +538,18 @@ intro orig.
 apply (shape_fun_full _ _ A C) in orig as shape. 2: reflexivity.
 destruct shape.
 + destruct H as [name [num]]. discriminate.
-+ destruct H. destruct H. destruct H. inv H. inv H0. apply TypeC; assumption.
++ do 3 (destruct H). inv H. inv H0. apply TypeC; assumption.
 Qed.
 
+
 (* ========================== Computation Shapes ========================== *)
+
 
 (* ΠMatch *)
 Fixpoint shape_prodmatch_full Γ c v x y c' C
   (orig : has_ctype Γ c C) {struct orig} :
   c = (ΠMatch v (x, y) c') ->
-  (exists A B, has_vtype Γ v (TyΠ A B) /\
-    has_ctype (CtxU (CtxU Γ A) B) c' C).
+  (exists A B, has_vtype Γ v (TyΠ A B) /\ has_ctype (CtxU (CtxU Γ A) B) c' C).
 Proof.  
 intros same. destruct orig. destruct H1; try discriminate.
 + clear shape_prodmatch_full. 
@@ -590,6 +562,7 @@ intros same. destruct orig. destruct H1; try discriminate.
   - assumption.
   - eapply TypeCSubtype. exact H1. assumption.
 Qed.
+
 
 Fixpoint shape_prodmatch Γ v x y c C :
   has_ctype Γ (ΠMatch v (x, y) c) C ->
@@ -622,6 +595,7 @@ intros same. destruct orig. destruct H1; try discriminate.
   - eapply TypeCSubtype. exact H4. assumption.
 Qed.
 
+
 Fixpoint shape_summatch Γ v xl cl xr cr C :
   has_ctype Γ (ΣMatch v xl cl xr cr) C ->
   (exists A B, has_vtype Γ v (TyΣ A B) /\
@@ -633,8 +607,7 @@ Qed.
 
 
 (* App *)
-Fixpoint shape_app_full Γ c x c' v C
-  (orig : has_ctype Γ c C) {struct orig} :
+Fixpoint shape_app_full Γ c x c' v C (orig : has_ctype Γ c C) {struct orig} :
   c = (App (Fun x c') v) ->
   (exists A, has_ctype (CtxU Γ A) c' C /\ has_vtype Γ v A).
 Proof.  
@@ -650,6 +623,7 @@ intros same. destruct orig. destruct H1; try discriminate.
   assumption. exact H4. exact H5. assumption.
 Qed.
 
+
 Fixpoint shape_app Γ x c v C :
   has_ctype Γ (App (Fun x c) v) C ->
   (exists A, has_ctype (CtxU Γ A) c C /\ has_vtype Γ v A).
@@ -657,3 +631,119 @@ Proof.
 intro orig. eapply (shape_app_full _ _ x c v C) in orig.
 2: reflexivity. assumption.
 Qed.
+
+
+(* LetRec *)
+Fixpoint shape_letrec_full Γ c f x c1 c2 D
+  (orig : has_ctype Γ c D) {struct orig} :
+  c = (LetRec f x c1 c2) ->
+  (exists A C, has_ctype (CtxU (CtxU Γ A) (TyFun A C)) c1 C /\ 
+  has_ctype (CtxU Γ (TyFun A C)) c2 D).
+Proof.  
+intros same. destruct orig. destruct H1; try discriminate.
++ clear shape_letrec_full. 
+  inv same. exists A. exists C. constructor; assumption.
++ apply (shape_letrec_full _ _ f x c1 c2) in H1;
+  clear shape_letrec_full. 2: assumption.
+  destruct H1 as [A' [C'' [cty]]].
+  exists A'. exists C''. constructor. assumption.
+  inv H1. apply TypeC; auto.
+  eapply TypeCSubtype. 2: exact H2. apply TypeC; assumption.
+Qed.
+
+
+Fixpoint shape_letrec Γ f x c1 c2 D :
+  has_ctype Γ (LetRec f x c1 c2) D ->
+  (exists A C, has_ctype (CtxU (CtxU Γ A) (TyFun A C)) c1 C /\ 
+    has_ctype (CtxU Γ (TyFun A C)) c2 D).
+Proof.
+intro orig. eapply (shape_letrec_full _ _ f x c1 c2 D) in orig.
+2: reflexivity. assumption.
+Qed.
+
+
+(* DoBind *)
+Fixpoint shape_dobind_full Γ c C x c1 c2 A Σ E
+  (orig : has_ctype Γ c C) {struct orig} :
+  c = (DoBind x c1 c2) -> C = (CTy A Σ E) ->
+  (exists A', has_ctype Γ c1 (CTy A' Σ E) /\ has_ctype (CtxU Γ A') c2 C).
+Proof.  
+intros same samety. destruct orig. destruct H1; try discriminate; inv same.
++ inv samety. clear shape_dobind_full. 
+  exists A0. constructor; assumption.
++ destruct C as (A', Σ', E').
+  apply (shape_dobind_full _ _ (CTy A' Σ' E') x c1 c2 A' Σ' E') in H1;
+  clear shape_dobind_full. 2: reflexivity. 2: reflexivity.
+  destruct H1 as [A'' [cty]].
+  exists A''. constructor.
+  - apply TypeC. assumption. inv cty. inv H0. inv H4.
+    apply WfCty; assumption. eapply TypeCSubtype. exact cty.
+     inv H2. inv cty. inv H3. 
+    apply Csubty. apply vsubtype_refl. all: assumption.
+  - apply TypeC. inv H1. assumption. assumption.
+    eapply TypeCSubtype. exact H1. assumption.
+Qed.
+
+
+Fixpoint shape_dobind Γ x c1 c2 A Σ E :
+  has_ctype Γ (DoBind x c1 c2) (CTy A Σ E) ->
+  (exists A', has_ctype Γ c1 (CTy A' Σ E) /\ 
+    has_ctype (CtxU Γ A') c2 (CTy A Σ E)).
+Proof.  
+intro orig. eapply (shape_dobind_full _ _ _ x c1 c2 A Σ E) in orig.
+2: reflexivity. assumption. reflexivity.
+Qed.
+
+
+(* Return *)
+Fixpoint shape_ret_full Γ c C v A Σ E
+  (orig : has_ctype Γ c C) {struct orig} :
+  c = (Ret v) -> C = (CTy A Σ E) -> has_vtype Γ v A.
+Proof.  
+intros same samety. destruct orig. destruct H1; try discriminate; inv same.
++ inv samety. assumption.
++ destruct C as (A', Σ', E').
+  apply (shape_ret_full _ _ (CTy A' Σ' E') v A' Σ' E') in H1;
+  clear shape_ret_full. 2: reflexivity. 2: reflexivity.
+  - apply TypeV. assumption. inv H0. assumption.
+    eapply TypeVSubtype. exact H1. inv H2. assumption.
+Qed.
+
+
+Fixpoint shape_ret Γ v A Σ E :
+  has_ctype Γ (Ret v) (CTy A Σ E) -> has_vtype Γ v A.
+Proof.  
+intro orig. eapply (shape_ret_full _ _ _ v A Σ E) in orig.
+2: reflexivity. assumption. reflexivity.
+Qed.
+
+(* Op
+Fixpoint shape_op_full Γ c C op v y c' A Σ E
+  (orig : has_ctype Γ c C) {struct orig} :
+  c = (Op op v y c') -> C = (CTy A Σ E) ->
+  (exists Aop Bop Aarg, get_op_type Σ op = Some (Aop, Bop) /\
+  has_vtype Γ v Aarg /\ vsubtype Aop Aarg /\ has_ctype (CtxU Γ Bop) c' C).
+Proof.  
+intros same samety. destruct orig. destruct H1; try discriminate; inv same.
++ inv samety. clear shape_op_full. 
+  exists A_op. exists B_op. exists A_op.
+  constructor. assumption. constructor. assumption.
+  constructor. apply vsubtype_refl. inv H2. assumption. assumption.
++ destruct C as (A', Σ', E').
+  apply (shape_op_full _ _ (CTy A' Σ' E') op v y c' A' Σ' E') in H1;
+  clear shape_op_full. 2: reflexivity. 2: reflexivity.
+  destruct H1 as [A'' [B'' [Aarg [g [vty]]]]]. 
+  inv H2. eapply sig_subtype_gets_Some in g. 2: exact H10.
+  destruct g as [A''' [B''' [g' [sty']]]].
+  exists A'''. exists B'''. exists Aarg. 
+  constructor. assumption. constructor. assumption.
+  constructor. eapply vsubtype_trans. exact sty'. destruct H1. assumption.
+  destruct H1. apply (ctx_subtype_ctype (CtxU Γ B'') (CtxU Γ B''')).
+  - apply TypeC. inv H3. assumption. assumption.
+    eapply TypeCSubtype. exact H3. apply Csubty; assumption.
+  - apply WfCtxU. assumption. apply get_op_type_wf in g'. destruct g'.
+    assumption. inv H0. assumption.
+  - apply CtxUsubty. apply ctx_subty_refl. assumption. assumption.
+
+Qed. *)
+
