language_formalisation/type_system/subtyping.v
@@ -24,8 +24,7 @@ with csubtype : ctype -> ctype -> Prop  :=
 with sig_subtype : sig -> sig -> Prop :=
 | SigØsubty Σ: sig_subtype SigØ Σ
 | SigUsubty Σ Σ' op A B A' B' : 
-    sig_subtype Σ Σ' -> 
-    get_op_type Σ op = None -> get_op_type Σ' op = Some (A', B') -> 
+    sig_subtype Σ Σ' -> get_op_type Σ' op = Some (A', B') -> 
     vsubtype A' A -> vsubtype B B' ->
     sig_subtype (SigU Σ op A B) Σ'
 
